$$
\emptyset\stackrel{\frac{\alpha\beta^i}{(1+\beta)^{i+1}}}\longrightarrow iP,i=1,2,3,...\\

N\stackrel{\tau}\Rightarrow\emptyset\tag{1}
$$

$G(z)=\Sigma z^mP(m)$

$G'(z)=\Sigma mz^{m-1}P(m)$

$G''(z)=\Sigma m(m-1)z^{m-2}P(m)$

$E(x)=\Sigma xP(x)=G'(1)$

$D(x)=E(x^2)-E(x)^2=x^2P(x)-[xP(x)]^2$

$G''(1)=\Sigma m^2P(m)-\Sigma mP(m)=\Sigma m^2P(m)-G'(1)$

$D(x)=G''(1)+G'(1)-[G'(1)]^2$

e.g for bursty model

$G(z)=\text{exp}(\frac{a\tau b(z-1)}{1-b(z-1)})$

$E(x)=\alpha\tau \beta$

$D(x)=\alpha\tau \beta+2\alpha\tau\beta^2$

if no delay occurs

$$
\emptyset\stackrel{\frac{\alpha\beta^i}{(1+\beta)^{i+1}}}\longrightarrow iP,i=1,2,3,...\\

P \xrightarrow {d}0 \tag{2}
$$

$E(x)=\frac{\alpha\beta}{d}$

$D(x)=\frac{\alpha\beta^2+\alpha\beta}{d}$
